thys/Native_Word/Uint8.thy
@@ -457,22 +457,12 @@ code_printing constant uint8_set_bit \<rightharpoonup>
   (Scala) "Uint8.set'_bit" and
   (Eval) "(fn x => fn i => fn b => if i < 0 orelse i >= 8 then raise (Fail \"argument to uint8'_set'_bit out of bounds\") else Uint8.set'_bit x i b)"
 
-
-definition uint8_shiftl :: "uint8 \<Rightarrow> integer \<Rightarrow> uint8"
-where [code del]:
-  "uint8_shiftl x n = (if n < 0 \<or> 8 \<le> n then undefined (push_bit :: nat \<Rightarrow> uint8 \<Rightarrow> _) x n else push_bit (nat_of_integer n) x)"
-
-lemma shiftl_uint8_code [code]:
-  "push_bit n x = (if n < 8 then uint8_shiftl x (integer_of_nat n) else 0)"
-  including undefined_transfer integer.lifting unfolding uint8_shiftl_def
-  by transfer simp
-
-lemma uint8_shiftl_code [code]:
-  "Rep_uint8 (uint8_shiftl w n) =
-  (if n < 0 \<or> 8 \<le> n then Rep_uint8 (undefined (push_bit :: nat \<Rightarrow> uint8 \<Rightarrow> _) w n)
-   else push_bit (nat_of_integer n) (Rep_uint8 w))"
-  including undefined_transfer unfolding uint8_shiftl_def
-  by transfer simp
+global_interpretation uint8: word_type_copy_target_language Abs_uint8 Rep_uint8 signed_drop_bit_uint8
+  uint8_of_nat nat_of_uint8 uint8_of_int int_of_uint8 Uint8 integer_of_uint8 8 set_bits_aux_uint8 8 7
+  defines uint8_shiftl = uint8.shiftl
+    and uint8_shiftr = uint8.shiftr
+    and uint8_sshiftr = uint8.sshiftr
+  by standard simp_all
 
 code_printing constant uint8_shiftl \<rightharpoonup>
   (SML) "Uint8.shiftl" and
@@ -480,44 +470,11 @@ code_printing constant uint8_shiftl \<rightharpoonup>
   (Scala) "Uint8.shiftl" and
   (Eval) "(fn x => fn i => if i < 0 orelse i >= 8 then raise (Fail \"argument to uint8'_shiftl out of bounds\") else Uint8.shiftl x i)"
 
-definition uint8_shiftr :: "uint8 \<Rightarrow> integer \<Rightarrow> uint8"
-where [code del]:
-  "uint8_shiftr x n = (if n < 0 \<or> 8 \<le> n then undefined (drop_bit :: _ \<Rightarrow> _ \<Rightarrow> uint8) x n else drop_bit (nat_of_integer n) x)"
-
-lemma shiftr_uint8_code [code]:
-  "drop_bit n x = (if n < 8 then uint8_shiftr x (integer_of_nat n) else 0)"
-  including undefined_transfer integer.lifting unfolding uint8_shiftr_def
-  by transfer simp
-
-lemma uint8_shiftr_code [code]:
-  "Rep_uint8 (uint8_shiftr w n) =
-  (if n < 0 \<or> 8 \<le> n then Rep_uint8 (undefined (drop_bit :: _ \<Rightarrow> _ \<Rightarrow> uint8) w n) 
-   else drop_bit (nat_of_integer n) (Rep_uint8 w))"
-including undefined_transfer unfolding uint8_shiftr_def by transfer simp
-
 code_printing constant uint8_shiftr \<rightharpoonup>
   (SML) "Uint8.shiftr" and
   (Haskell) "Data'_Bits.shiftrBounded" and
   (Scala) "Uint8.shiftr" and
   (Eval) "(fn x => fn i => if i < 0 orelse i >= 8 then raise (Fail \"argument to uint8'_shiftr out of bounds\") else Uint8.shiftr x i)"
-
-definition uint8_sshiftr :: "uint8 \<Rightarrow> integer \<Rightarrow> uint8"
-where [code del]:
-  "uint8_sshiftr x n =
-  (if n < 0 \<or> 8 \<le> n then undefined signed_drop_bit_uint8 n x else signed_drop_bit_uint8 (nat_of_integer n) x)"
-
-lemma sshiftr_uint8_code [code]:
-  "signed_drop_bit_uint8 n x = 
-  (if n < 8 then uint8_sshiftr x (integer_of_nat n) else if bit x 7 then -1 else 0)"
-  including undefined_transfer integer.lifting unfolding uint8_sshiftr_def
-  by transfer (simp add: not_less signed_drop_bit_beyond word_size)
-
-lemma uint8_sshiftr_code [code]:
-  "Rep_uint8 (uint8_sshiftr w n) =
-  (if n < 0 \<or> 8 \<le> n then Rep_uint8 (undefined signed_drop_bit_uint8 n w)
-   else signed_drop_bit (nat_of_integer n) (Rep_uint8 w))"
-  including undefined_transfer unfolding uint8_sshiftr_def
-  by transfer simp
 
 code_printing constant uint8_sshiftr \<rightharpoonup>
   (SML) "Uint8.shiftr'_signed" and
